Generalize pattern 6 and add proofs for Barrier

Pattern2_Def.thy
@@ -8,8 +8,8 @@ definition previous_all where " previous_all s A \<equiv>
 definition previous_ex where "previous_ex s A \<equiv>
 \<exists> s1. consecutive s1 s \<and> A s1"
 
-definition always2 where  "always2 s A1 A2 \<equiv> 
-\<forall> s1 s2. substate s1 s2 \<and> substate s2 s \<and> toEnvP s1 \<and> toEnvP s2 \<and> toEnvNum s1 s2 = 1 \<and> A1 s1 s2 \<longrightarrow> A2 s2"
+definition always2 where  "always2 s A1 A2 A3 \<equiv> 
+always s (\<lambda> s2.( previous_ex s2 A1) \<and> A2 s2 \<longrightarrow> A3 s2)"
 
 lemma previous_all_one_point: "consecutive s0 s \<Longrightarrow>  A s0 \<Longrightarrow> previous_all s A"
   apply(unfold  previous_all_def)
@@ -33,11 +33,14 @@ lemma previous_ex_rule: "
   by (meson consecutive.simps substate_trans)
 
 lemma always2_rule: "consecutive s0 s \<Longrightarrow>
-always2 s0 A1 A2 \<and> (\<not> A1 s0 s \<or> A2' s) \<and> (\<forall> s1. toEnvP s1 \<and> substate s1 s0 \<and> A2 s1 \<longrightarrow> A2' s1) \<Longrightarrow> always2 s A1 A2'"
+always2 s0 A1 A2 A3 \<and> (\<not> A1 s0 \<or> ~ A2 s \<or> A3' s) \<and> (\<forall> s1. toEnvP s1 \<and> substate s1 s0 \<and> A3 s1 \<longrightarrow> A3' s1) \<Longrightarrow> always2 s A1 A2 A3'"
   apply(unfold always2_def)
-  by (metis consecutive.elims(2) substate_noteq_imp_substate_of_pred toEnvNum_eq_imp_eq2)
+  by (smt (verit) always_def consecutive.elims(2) previous_ex_def substate_noteq_imp_substate_of_pred toEnvNum_eq_imp_eq2)
 
-lemma always2_einv2req: "always2 s A1 A2 \<and>  (\<forall> s1. toEnvP s1 \<and> substate s1 s \<and> A2 s1 \<longrightarrow> A2' s1) \<Longrightarrow> always2 s A1 A2'"
-  using always2_def by auto
+
+
+lemma always2_einv2req: "always2 s A1 A2 A3 \<and>  (\<forall> s1. toEnvP s1 \<and> substate s1 s \<and> A3 s1 \<longrightarrow> A3' s1) \<Longrightarrow> always2 s A1 A2 A3'"
+  apply(unfold always2_def)
+  by (simp add: always_def)
 
 end
