Pattern3_Def.thy
@@ -3,12 +3,13 @@ theory Pattern3_Def
 begin
 
 definition always where "always s A \<equiv>
-\<forall> s1. substate s1 s \<and> toEnvP s1 \<and> A s1"
+\<forall> s1. substate s1 s \<and> toEnvP s1 \<longrightarrow> A s1"
 
 lemma always_rule: "always s0 A \<and> (A' s) \<and> (\<forall> s1 . toEnvP s1 \<and> substate s1 s0 \<and>A s1 \<longrightarrow> A' s1) \<Longrightarrow>
 consecutive s0 s \<Longrightarrow> always s A'"
   apply(unfold always_def)
-  using substate_antisym by auto
+  by (metis consecutive.elims(2) substate_noteq_imp_substate_of_pred)
+
 
 lemma always_einv2req: " always s A \<and>  (\<forall> s1 . toEnvP s1 \<and> substate s1 s \<and>A s1 \<longrightarrow> A' s1) \<Longrightarrow>
   always s A'"
