Barrier/Proofs_R3.thy
@@ -1,0 +1,180 @@
+theory Proofs_R3
+  imports ExtraInv_R3 Requirements
+begin
+
+definition inv3 where "inv3 s \<equiv> extraInv2 s \<and> R3 s"
+
+theorem "VC1 inv3 s0"
+  apply(unfold VC1_def inv3_def R3_def P6_2_def always2_def always_def weak_until_def previous_ex_def)
+  using extra1 VC1_def apply auto
+  done
+
+theorem "VC2 inv3 env s0 carInFront'value peCarUnder'value opened'value closed'value"
+  apply(unfold VC2_def inv3_def R3_def)
+  apply(rule impI)
+  apply(rule context_conjI)
+  using extra2 VC2_def apply auto[1]
+  apply(rule conjI)
+   apply simp
+  apply(unfold extraInv2_def commonExtraInv_def)
+  apply(erule conjE)+
+  apply(auto simp add:  P6_2_einv2req)
+  done
+
+theorem "VC3 inv3 env s0 carInFront'value peCarUnder'value opened'value closed'value"
+  apply(unfold VC3_def inv3_def R3_def)
+  apply(rule impI)
+  apply(rule context_conjI)
+  using extra3 VC3_def apply auto[1]
+  apply(rule conjI)
+   apply simp
+  apply(unfold extraInv2_def commonExtraInv_def)
+  apply(erule conjE)+
+  apply(auto simp add:  P6_2_einv2req)
+  done
+
+theorem "VC4 inv3 env s0 carInFront'value peCarUnder'value opened'value closed'value"
+  apply(unfold VC4_def inv3_def R3_def)
+  apply(rule impI)
+  apply(rule context_conjI)
+  using extra4 VC4_def apply auto[1]
+  apply(rule conjI)
+   apply simp
+  apply(unfold extraInv2_def commonExtraInv_def)
+  apply(erule conjE)+
+  apply(auto simp add:  P6_2_einv2req)
+  done
+
+theorem "VC14 inv3 env s0 carInFront'value peCarUnder'value opened'value closed'value"
+  apply(unfold VC14_def inv3_def R3_def)
+  apply(rule impI)
+  apply(rule context_conjI)
+  using extra14 VC14_def apply auto[1]
+  apply(rule conjI)
+   apply simp
+  apply(unfold extraInv2_def commonExtraInv_def)
+  apply(erule conjE)+
+  apply(auto simp add:  P6_2_einv2req)
+  done
+
+theorem "VC15 inv3 env s0 carInFront'value peCarUnder'value opened'value closed'value"
+  apply(unfold VC15_def inv3_def R3_def)
+  apply(rule impI)
+  apply(rule context_conjI)
+  using extra15 VC15_def apply auto[1]
+  apply(rule conjI)
+   apply simp
+  apply(unfold extraInv2_def commonExtraInv_def)
+  apply(erule conjE)+
+  apply(auto simp add:  P6_2_einv2req)
+  done
+
+theorem "VC16 inv3 env s0 carInFront'value peCarUnder'value opened'value closed'value"
+  apply(unfold VC16_def inv3_def R3_def)
+  apply(rule impI)
+  apply(rule context_conjI)
+  using extra16 VC16_def apply auto[1]
+  apply(rule conjI)
+   apply simp
+  apply(unfold extraInv2_def commonExtraInv_def)
+  apply(erule conjE)+
+  apply(auto simp add:  P6_2_einv2req)
+  done
+
+theorem "VC17 inv3 env s0 carInFront'value peCarUnder'value opened'value closed'value"
+  apply(unfold VC17_def inv3_def R3_def)
+  apply(rule impI)
+  apply(rule context_conjI)
+  using extra17 VC17_def apply auto[1]
+  apply(rule conjI)
+   apply simp
+  apply(unfold extraInv2_def commonExtraInv_def)
+  apply(erule conjE)+
+  apply(auto simp add:  P6_2_einv2req)
+  done
+
+theorem "VC18 inv3 env s0 carInFront'value peCarUnder'value opened'value closed'value"
+  apply(unfold VC18_def inv3_def R3_def)
+  apply(rule impI)
+  apply(rule context_conjI)
+  using extra18 VC18_def apply auto[1]
+  apply(rule conjI)
+   apply simp
+  apply(unfold extraInv2_def commonExtraInv_def)
+  apply(erule conjE)+
+  apply(auto simp add:  P6_2_einv2req)
+  done
+
+theorem "VC19 inv3 env s0 carInFront'value peCarUnder'value opened'value closed'value"
+  apply(unfold VC19_def inv3_def R3_def)
+  apply(rule impI)
+  apply(rule context_conjI)
+  using extra19 VC19_def apply auto[1]
+  apply(rule conjI)
+   apply simp
+  apply(unfold extraInv2_def commonExtraInv_def)
+  apply(erule conjE)+
+  apply(auto simp add:  P6_2_einv2req)
+  done
+
+theorem "VC20 inv3 env s0 carInFront'value peCarUnder'value opened'value closed'value"
+  apply(unfold VC20_def inv3_def R3_def)
+  apply(rule impI)
+  apply(rule context_conjI)
+  using extra20 VC20_def apply auto[1]
+  apply(rule conjI)
+   apply simp
+  apply(unfold extraInv2_def commonExtraInv_def)
+  apply(erule conjE)+
+  apply(auto simp add:  P6_2_einv2req)
+  done
+
+theorem "VC21 inv3 env s0 carInFront'value peCarUnder'value opened'value closed'value"
+  apply(unfold VC21_def inv3_def R3_def)
+  apply(rule impI)
+  apply(rule context_conjI)
+  using extra21 VC21_def apply auto[1]
+  apply(rule conjI)
+   apply simp
+  apply(unfold extraInv2_def commonExtraInv_def)
+  apply(erule conjE)+
+  apply(auto simp add:  P6_2_einv2req)
+  done
+
+theorem "VC22 inv3 env s0 carInFront'value peCarUnder'value opened'value closed'value"
+  apply(unfold VC22_def inv3_def R3_def)
+  apply(rule impI)
+  apply(rule context_conjI)
+  using extra22 VC22_def apply auto[1]
+  apply(rule conjI)
+   apply simp
+  apply(unfold extraInv2_def commonExtraInv_def)
+  apply(erule conjE)+
+  apply(auto simp add:  P6_2_einv2req)
+  done
+
+theorem "VC23 inv3 env s0 carInFront'value peCarUnder'value opened'value closed'value"
+  apply(unfold VC23_def inv3_def R3_def)
+  apply(rule impI)
+  apply(rule context_conjI)
+  using extra23 VC23_def apply auto[1]
+  apply(rule conjI)
+   apply simp
+  apply(unfold extraInv2_def commonExtraInv_def)
+  apply(erule conjE)+
+  apply(auto simp add:  P6_2_einv2req)
+  done
+
+theorem "VC24 inv3 env s0 carInFront'value peCarUnder'value opened'value closed'value"
+  apply(unfold VC24_def inv3_def R3_def)
+  apply(rule impI)
+  apply(rule context_conjI)
+  using extra24 VC24_def apply auto[1]
+  apply(rule conjI)
+   apply simp
+  apply(unfold extraInv2_def commonExtraInv_def)
+  apply(erule conjE)+
+  apply(auto simp add:  P6_2_einv2req)
+  done
+
+end
